**Parabola:**
$$
y = ax^2 + bx + c
$$

**Y-axis:**
$$
y = a \cdot 0^2 + b \cdot 0 + c \quad (0, c)
$$

<br>

**X-axis:**
$$
0 = ax^2 + bx + c
$$

$$
x^2 + \frac{bx}{a} + \frac{c}{a} = 0
$$

$$
x^2 + \frac{bx}{a} \cdot \frac{1}{2} + \frac{c}{a} = 0
$$

$$
\left(x + \frac{b}{2a}\right)^2 + \frac{c}{a} \Rightarrow x^2 + \frac{bx}{2a} + \frac{b^2}{4a^2} + \frac{c}{a}
$$

$$
\Rightarrow x^2 + \frac{bx}{a} + \frac{b^2}{4a^2} - \frac{b^2}{4a^2} + \frac{c}{a}
$$

$$
\Rightarrow \left(x + \frac{b}{2a}\right)^2 - \left(\frac{b}{2a}\right)^2 + \frac{c}{a}
$$

$$
\Rightarrow \left(x + \frac{b}{2a}\right)^2 = \left(\frac{b}{2a}\right)^2 - \frac{c}{a}
$$

$$
\Rightarrow x + \frac{b}{2a} = \pm \sqrt{\frac{b^2}{4a^2} - \frac{c}{a}}
$$

$$
\Rightarrow x = -\frac{b}{2a} \pm \sqrt{\frac{b^2}{4a^2} - \frac{c}{a}}
$$

$$
\Rightarrow x = \frac{-b \pm \sqrt{b^2 - 4ac}}{2a}
$$

**Parabola:**
$$
y = dx^2 + fx + g
$$

**Y-axis:**
$$
y = d \cdot 0^2 + f \cdot 0 + g \quad (0, g)
$$

<br>

**X-axis:**
$$
0 = dx^2 + fx + g
$$

$$
x^2 + \frac{fx}{d} + \frac{g}{d} = 0
$$

$$
x^2 + \frac{fx}{d} \cdot \frac{1}{2} + \frac{g}{d} = 0
$$

$$
\left(x + \frac{f}{2d}\right)^2 + \frac{g}{d} \Rightarrow x^2 + \frac{fx}{2d} + \frac{f^2}{4d^2} + \frac{g}{d}
$$

$$
\Rightarrow x^2 + \frac{fx}{d} + \frac{f^2}{4d^2} - \frac{f^2}{4d^2} + \frac{g}{d}
$$

$$
\Rightarrow \left(x + \frac{f}{2d}\right)^2 - \left(\frac{f}{2d}\right)^2 + \frac{g}{d}
$$

$$
\Rightarrow \left(x + \frac{f}{2d}\right)^2 = \left(\frac{f}{2d}\right)^2 - \frac{g}{d}
$$

$$
\Rightarrow x + \frac{f}{2d} = \pm \sqrt{\frac{f^2}{4d^2} - \frac{g}{d}}
$$

$$
\Rightarrow x = -\frac{f}{2d} \pm \sqrt{\frac{f^2}{4d^2} - \frac{g}{d}}
$$

$$
\Rightarrow x = \frac{-f \pm \sqrt{f^2 - 4dg}}{2d}
$$
